Multiplication based on prime

code/ecdsa/dist/Hacl_P256.c
@@ -42,31 +42,6 @@ prime384_buffer[6U] =
     (uint64_t)0xffffffffffffffffU, (uint64_t)0xffffffffffffffffU, (uint64_t)0xffffffffffffffffU
   };
 
-static const
-uint8_t
-prime256_inverse_buffer[32U] =
-  {
-    (uint8_t)253U, (uint8_t)255U, (uint8_t)255U, (uint8_t)255U, (uint8_t)255U, (uint8_t)255U,
-    (uint8_t)255U, (uint8_t)255U, (uint8_t)255U, (uint8_t)255U, (uint8_t)255U, (uint8_t)255U,
-    (uint8_t)0U, (uint8_t)0U, (uint8_t)0U, (uint8_t)0U, (uint8_t)0U, (uint8_t)0U, (uint8_t)0U,
-    (uint8_t)0U, (uint8_t)0U, (uint8_t)0U, (uint8_t)0U, (uint8_t)0U, (uint8_t)1U, (uint8_t)0U,
-    (uint8_t)0U, (uint8_t)0U, (uint8_t)255U, (uint8_t)255U, (uint8_t)255U, (uint8_t)255U
-  };
-
-static const
-uint8_t
-prime384_inverse_buffer[48U] =
-  {
-    (uint8_t)253U, (uint8_t)255U, (uint8_t)255U, (uint8_t)255U, (uint8_t)0U, (uint8_t)0U,
-    (uint8_t)0U, (uint8_t)0U, (uint8_t)0U, (uint8_t)0U, (uint8_t)0U, (uint8_t)0U, (uint8_t)255U,
-    (uint8_t)255U, (uint8_t)255U, (uint8_t)255U, (uint8_t)254U, (uint8_t)255U, (uint8_t)255U,
-    (uint8_t)255U, (uint8_t)255U, (uint8_t)255U, (uint8_t)255U, (uint8_t)255U, (uint8_t)255U,
-    (uint8_t)255U, (uint8_t)255U, (uint8_t)255U, (uint8_t)255U, (uint8_t)255U, (uint8_t)255U,
-    (uint8_t)255U, (uint8_t)255U, (uint8_t)255U, (uint8_t)255U, (uint8_t)255U, (uint8_t)255U,
-    (uint8_t)255U, (uint8_t)255U, (uint8_t)255U, (uint8_t)255U, (uint8_t)255U, (uint8_t)255U,
-    (uint8_t)255U, (uint8_t)255U, (uint8_t)255U, (uint8_t)255U, (uint8_t)255U
-  };
-
 static inline uint64_t
 mul_carry_add_u64_st(uint64_t c_in, uint64_t a, uint64_t b, uint64_t *out)
 {
@@ -2330,16 +2305,17 @@ static void montgomery_square_buffer_k0(Spec_P256_curve c, uint64_t *a, uint64_t
 static void
 montgomery_multiplication_buffer_by_one(Spec_P256_curve c, uint64_t *a, uint64_t *result)
 {
+  const uint64_t *primeBuffer;
   switch (c)
   {
     case Spec_P256_P256:
       {
-        montgomery_multiplication_buffer_by_one_w_ko(c, a, result);
+        primeBuffer = prime256_buffer;
         break;
       }
     case Spec_P256_P384:
       {
-        montgomery_multiplication_buffer_by_one_ko(c, a, result);
+        primeBuffer = prime384_buffer;
         break;
       }
     default:
@@ -2348,6 +2324,13 @@ montgomery_multiplication_buffer_by_one(Spec_P256_curve c, uint64_t *a, uint64_t
         KRML_HOST_EXIT(253U);
       }
   }
+  uint64_t primeBuffer0 = primeBuffer[0U];
+  if (primeBuffer0 == (uint64_t)0xffffffffffffffffU)
+  {
+    montgomery_multiplication_buffer_by_one_w_ko(c, a, result);
+    return;
+  }
+  montgomery_multiplication_buffer_by_one_ko(c, a, result);
 }
 
 static void
@@ -2403,164 +2386,50 @@ static void fsquarePowN(Spec_P256_curve c, uint32_t n, uint64_t *a)
   }
 }
 
-static inline void cswap(Spec_P256_curve c, uint64_t bit, uint64_t *p1, uint64_t *p2)
+static inline void exponent_p384(uint64_t *t, uint64_t *result, uint64_t *tempBuffer)
 {
-  uint64_t mask = (uint64_t)0U - bit;
-  uint32_t len;
-  switch (c)
-  {
-    case Spec_P256_P256:
-      {
-        len = (uint32_t)4U;
-        break;
-      }
-    case Spec_P256_P384:
-      {
-        len = (uint32_t)6U;
-        break;
-      }
-    default:
-      {
-        len = (uint32_t)4U;
-      }
-  }
-  for (uint32_t i = (uint32_t)0U; i < len; i++)
-  {
-    uint64_t dummy = mask & (p1[i] ^ p2[i]);
-    p1[i] = p1[i] ^ dummy;
-    p2[i] = p2[i] ^ dummy;
-  }
-}
-
-static void
-montgomery_ladder_power_step(
-  Spec_P256_curve c,
-  uint64_t *a,
-  uint64_t *b,
-  const uint8_t *scalar,
-  uint32_t i
-)
-{
-  uint32_t sw;
-  switch (c)
-  {
-    case Spec_P256_P256:
-      {
-        sw = (uint32_t)32U;
-        break;
-      }
-    case Spec_P256_P384:
-      {
-        sw = (uint32_t)48U;
-        break;
-      }
-    default:
-      {
-        KRML_HOST_EPRINTF("KreMLin incomplete match at %s:%d\n", __FILE__, __LINE__);
-        KRML_HOST_EXIT(253U);
-      }
-  }
-  uint32_t bit0 = sw * (uint32_t)8U - (uint32_t)1U - i;
-  uint64_t bit = (uint64_t)(scalar[bit0 / (uint32_t)8U] >> bit0 % (uint32_t)8U & (uint8_t)1U);
-  cswap(c, bit, a, b);
-  montgomery_multiplication_buffer(c, a, b, b);
-  montgomery_square_buffer(c, a, a);
-  cswap(c, bit, a, b);
-}
-
-static void
-_montgomery_ladder_power(Spec_P256_curve c, uint64_t *a, uint64_t *b, const uint8_t *scalar)
-{
-  uint32_t sw;
-  switch (c)
-  {
-    case Spec_P256_P256:
-      {
-        sw = (uint32_t)32U;
-        break;
-      }
-    case Spec_P256_P384:
-      {
-        sw = (uint32_t)48U;
-        break;
-      }
-    default:
-      {
-        KRML_HOST_EPRINTF("KreMLin incomplete match at %s:%d\n", __FILE__, __LINE__);
-        KRML_HOST_EXIT(253U);
-      }
-  }
-  uint32_t scalarLen = sw * (uint32_t)8U;
-  for (uint32_t i = (uint32_t)0U; i < scalarLen; i++)
-  {
-    montgomery_ladder_power_step(c, a, b, scalar, i);
-  }
-}
-
-static void
-montgomery_ladder_power(
-  Spec_P256_curve c,
-  uint64_t *a,
-  const uint8_t *scalar,
-  uint64_t *result
-)
-{
-  uint32_t len;
-  switch (c)
-  {
-    case Spec_P256_P256:
-      {
-        len = (uint32_t)4U;
-        break;
-      }
-    case Spec_P256_P384:
-      {
-        len = (uint32_t)6U;
-        break;
-      }
-    default:
-      {
-        len = (uint32_t)4U;
-      }
-  }
-  KRML_CHECK_SIZE(sizeof (uint64_t), len);
-  uint64_t p[len];
-  memset(p, 0U, len * sizeof (uint64_t));
-  switch (c)
-  {
-    case Spec_P256_P256:
-      {
-        p[0U] = (uint64_t)1U;
-        p[1U] = (uint64_t)18446744069414584320U;
-        p[2U] = (uint64_t)18446744073709551615U;
-        p[3U] = (uint64_t)4294967294U;
-        break;
-      }
-    default:
-      {
-        reduction_prime_2prime_with_carry_cin(c, (uint64_t)1U, p, p);
-      }
-  }
-  _montgomery_ladder_power(c, p, a, scalar);
-  uint32_t sw;
-  switch (c)
-  {
-    case Spec_P256_P256:
-      {
-        sw = (uint32_t)4U;
-        break;
-      }
-    case Spec_P256_P384:
-      {
-        sw = (uint32_t)6U;
-        break;
-      }
-    default:
-      {
-        sw = (uint32_t)4U;
-      }
-  }
-  memcpy(result, p, sw * sizeof (uint64_t));
+  uint64_t *t0 = tempBuffer;
+  uint64_t *t1 = tempBuffer + (uint32_t)6U;
+  uint64_t *t2 = tempBuffer + (uint32_t)12U;
+  uint64_t *t3 = tempBuffer + (uint32_t)18U;
+  uint64_t *t4 = tempBuffer + (uint32_t)24U;
+  uint64_t *t5 = tempBuffer + (uint32_t)30U;
+  montgomery_square_buffer(Spec_P256_P384, t, t0);
+  montgomery_multiplication_buffer(Spec_P256_P384, t, t0, t0);
+  montgomery_square_buffer(Spec_P256_P384, t0, t0);
+  montgomery_multiplication_buffer(Spec_P256_P384, t, t0, t0);
+  montgomery_square_buffer(Spec_P256_P384, t0, t1);
+  fsquarePowN(Spec_P256_P384, (uint32_t)2U, t1);
+  montgomery_multiplication_buffer(Spec_P256_P384, t0, t1, t1);
+  montgomery_square_buffer(Spec_P256_P384, t1, t2);
+  fsquarePowN(Spec_P256_P384, (uint32_t)5U, t2);
+  montgomery_multiplication_buffer(Spec_P256_P384, t2, t1, t2);
+  montgomery_square_buffer(Spec_P256_P384, t2, t3);
+  fsquarePowN(Spec_P256_P384, (uint32_t)11U, t3);
+  montgomery_multiplication_buffer(Spec_P256_P384, t2, t3, t2);
+  fsquarePowN(Spec_P256_P384, (uint32_t)6U, t2);
+  montgomery_multiplication_buffer(Spec_P256_P384, t2, t1, t1);
+  montgomery_square_buffer(Spec_P256_P384, t1, t2);
+  montgomery_multiplication_buffer(Spec_P256_P384, t2, t, t2);
+  montgomery_square_buffer(Spec_P256_P384, t2, t3);
+  montgomery_multiplication_buffer(Spec_P256_P384, t, t3, t3);
+  montgomery_square_buffer(Spec_P256_P384, t3, t4);
+  fsquarePowN(Spec_P256_P384, (uint32_t)30U, t4);
+  montgomery_multiplication_buffer(Spec_P256_P384, t4, t2, t4);
+  montgomery_square_buffer(Spec_P256_P384, t4, t5);
+  fsquarePowN(Spec_P256_P384, (uint32_t)62U, t5);
+  montgomery_multiplication_buffer(Spec_P256_P384, t4, t5, t4);
+  montgomery_square_buffer(Spec_P256_P384, t4, t5);
+  fsquarePowN(Spec_P256_P384, (uint32_t)125U, t5);
+  montgomery_multiplication_buffer(Spec_P256_P384, t4, t5, t4);
+  fsquarePowN(Spec_P256_P384, (uint32_t)3U, t4);
+  montgomery_multiplication_buffer(Spec_P256_P384, t4, t0, t4);
+  fsquarePowN(Spec_P256_P384, (uint32_t)33U, t4);
+  montgomery_multiplication_buffer(Spec_P256_P384, t4, t3, t4);
+  fsquarePowN(Spec_P256_P384, (uint32_t)94U, t4);
+  montgomery_multiplication_buffer(Spec_P256_P384, t4, t1, t4);
+  fsquarePowN(Spec_P256_P384, (uint32_t)2U, t4);
+  montgomery_multiplication_buffer(Spec_P256_P384, t4, t, result);
 }
 
 static inline void exponent_p256(uint64_t *t, uint64_t *result, uint64_t *tempBuffer)
@@ -2612,26 +2481,7 @@ static void exponent(Spec_P256_curve c, uint64_t *a, uint64_t *result, uint64_t 
   {
     case Spec_P256_P384:
       {
-        const uint8_t *sw;
-        switch (c)
-        {
-          case Spec_P256_P256:
-            {
-              sw = prime256_inverse_buffer;
-              break;
-            }
-          case Spec_P256_P384:
-            {
-              sw = prime384_inverse_buffer;
-              break;
-            }
-          default:
-            {
-              KRML_HOST_EPRINTF("KreMLin incomplete match at %s:%d\n", __FILE__, __LINE__);
-              KRML_HOST_EXIT(253U);
-            }
-        }
-        montgomery_ladder_power(c, a, sw, result);
+        exponent_p384(a, result, tempBuffer);
         break;
       }
     case Spec_P256_P256:
@@ -4858,7 +4708,7 @@ static uint64_t isPointAtInfinityPrivate(Spec_P256_curve c, uint64_t *p)
   return r;
 }
 
-static inline void cswap0(Spec_P256_curve c, uint64_t bit, uint64_t *p1, uint64_t *p2)
+static inline void cswap(Spec_P256_curve c, uint64_t bit, uint64_t *p1, uint64_t *p2)
 {
   uint64_t mask = (uint64_t)0U - bit;
   uint32_t sw;
@@ -5160,9 +5010,9 @@ montgomery_ladder_step(
   }
   uint32_t bit0 = sw - i - (uint32_t)1U;
   uint64_t bit = scalar_bit(c, buf_type, scalar, bit0);
-  cswap0(c, bit, r0, r1);
+  cswap(c, bit, r0, r1);
   montgomery_ladder_step1(c, r0, r1, tempBuffer);
-  cswap0(c, bit, r0, r1);
+  cswap(c, bit, r0, r1);
 }
 
 static void
